RiseLean/TestSyntax.lean
@@ -1,0 +1,23 @@
+import Lean
+import RiseLean.DataType
+open Lean Elab Meta Command Term
+
+/--
+  Utility elaborator for Rise Types - adds metavariables to context.
+  "[Rise Type with <identifiers> | <rise_type>]"
+
+  TODO (if necessary): make a difference between variables and metavariables.
+  TODO (if necessary): currently all metavars are just data
+-/
+elab "[RTw" mvars:ident* "|" t:rise_type "]" : term => do
+  let l ← liftMacroM <| expandMacros t
+  let kctx : RKindingCtx := #[]
+  let mctx_list ← mvars.toList.mapM (fun var => do
+    let name := var.getId
+    let kind_expr ← `(RKind.data)
+    let kind_elab ← elabTerm kind_expr none
+    return (name, kind_elab)
+  )
+  let mctx := mctx_list.toArray
+  elabRType kctx mctx l
+
